define semantics

TAPLFormalization/02-lambda/AST.lean
@@ -10,24 +10,17 @@ def FV : LambdaTerm → Std.HashSet String
   | .abs arg body => (FV body).erase arg
   | .app t₁ t₂ => (FV t₁).union (FV t₂)
 
-abbrev NamingContext := List String
-
 inductive IndexedTerm where
-  | var (k : ℕ) : IndexedTerm
-  | abs (body : IndexedTerm) : IndexedTerm
+  | freeV (name : String) : IndexedTerm
+  | boundV (index : ℕ) : IndexedTerm
   | app (t₁ t₂ : IndexedTerm) : IndexedTerm
+  | abs (body : IndexedTerm) : IndexedTerm
 
-inductive NIndexedTerm : (n : ℕ) → IndexedTerm → Prop where
-  | var (k : ℕ) : (k ≤ n) → NIndexedTerm n (.var k)
-  | abs (body : IndexedTerm) : NIndexedTerm (n+1) body → NIndexedTerm n (.abs body)
-  | app (t₁ t₂ : IndexedTerm) : NIndexedTerm n t₁ → NIndexedTerm n t₂ → NIndexedTerm n (.app t₁ t₂)
+def removeNames' (depth : ℕ) (levels : Std.HashMap String ℕ) : LambdaTerm → IndexedTerm
+  | .var name => match levels[name]? with
+    | .some k => .boundV k
+    | .none => .freeV name
+  | .abs arg body => .abs (removeNames' (depth + 1) (levels.insert arg depth) body)
+  | .app t₁ t₂ => .app (removeNames' depth levels t₁) (removeNames' depth levels t₂)
 
-def removeNames (Γ : NamingContext) (t : LambdaTerm) (h_in : ∀ x ∈ FV t, Γ.contains x) : {it : IndexedTerm // NIndexedTerm Γ.length it} := by
-  cases t with
-  | var x =>
-    let it := IndexedTerm.var (Γ.findIdx (· == x))
-    exists it
-    constructor
-    let x_in_Γ := h_in x (by simp [FV, Std.HashSet.ofList, Std.HashSet.instMembership])
-
-    sorry
+def removeNames := removeNames' 0 ∅
