TAPLFormalization/02-lambda/Programming.lean
@@ -1,3 +1,28 @@
-import TAPLFormalization.«02-lambda».AST
+import TAPLFormalization.«02-lambda».Semantics
 
---
+infixl:100 "|$|" => LambdaTerm.app
+abbrev la := LambdaTerm.abs
+instance : Coe String LambdaTerm where
+  coe := .var
+
+-- Church booleans, numerals, recursion, etc.
+def cTrue : LambdaTerm := la "x" $ la "y" $ "x"
+def cFalse : LambdaTerm := la "x" $ la "y" $ "y"
+def cNot : LambdaTerm := la "b" $ la "x" $ la "y" $ "b" |$| "y" |$| "x"
+def cOr : LambdaTerm := la "a" $ la "b" $ "a" |$| cTrue |$| ("b" |$| cTrue |$| cFalse)
+def cAnd : LambdaTerm := la "a" $ la "b" $ "a" |$| ("b" |$| cTrue |$| cFalse) |$| cFalse
+
+infix:100 " ~> " => CV.SmallStep
+def cId : LambdaTerm := la "x" "x"
+
+example : CV.SmallSteps (removeNames $ cId |$| (cId |$| (la "z" (cId |$| "z")))) (removeNames $ la "z" $ cId |$| "z") := by
+  calc
+    _ ~> (removeNames $ cId |$| (la "z" (cId |$| "z"))) := by
+      simp [removeNames, removeNames', cId]
+      apply CV.SmallStep.appArg
+      apply CV.SmallStep.appAbs
+      simp [subst, subst', addDepth]
+    _ ~> _ := by
+      simp [removeNames, removeNames', cId]
+      apply CV.SmallStep.appAbs
+      simp [subst, subst', addDepth]
